src/Equivalence/Basics.v
@@ -1,0 +1,28 @@
+From CoreErlang Require Export Basics.
+Require Export stdpp.list.
+
+(**
+NOTES:  Maybe place this in CoreErlang/Basics
+*)
+
+
+
+Lemma foldl_ext :
+  forall (A B : Type) (f1 f2 : A -> B -> A) (x1 x2 : A) (l1 l2 : list B),
+    (forall (a : A) (b : B), f1 a b = f2 a b) ->
+    l1 = l2 ->
+    x1 = x2 ->
+    fold_left f1 l1 x1 = fold_left f2 l2 x2.
+Proof.
+  intros A B f1 f2 x1 x2 l1 l2 Hf Hl Hx.
+  rewrite Hl.
+  rewrite Hx.
+  clear Hl Hx l1 x1.
+  rename l2 into l.
+  rename x2 into x.
+  revert x.
+  induction l as [| b l IHl]; intros x; simpl.
+  - reflexivity.
+  - rewrite Hf.
+    by rewrite IHl.
+Qed.
