src/Equivalence/BigStepToFrameStack/EnvironmentDefinitions.v
@@ -1,0 +1,86 @@
+From CoreErlang.BigStep Require Export Environment.
+
+(**
+* Help
+  - env_rem
+* Main
+  - env_rem_vars
+  - env_rem_fids
+  - env_rem_fids_vars
+  - env_rem_ext
+*)
+
+(**
+NOTES:  Maybe place this in BigStep/Environment
+*)
+
+
+
+Section Help.
+
+
+
+  Definition env_rem
+    (keys : list (Var + FunctionIdentifier))
+    (env : Environment)
+    : Environment
+    :=
+  fold_left
+    (fun env' key =>
+      filter (fun '(k, v) =>
+        negb (var_funid_eqb k key))
+        env')
+    keys
+    env.
+
+
+
+End Help.
+
+
+
+
+
+
+Section Main.
+
+
+
+  Definition env_rem_vars
+    (vars : list Var)
+    (env : Environment)
+    : Environment
+    :=
+  env_rem (map inl vars) env.
+
+
+
+  Definition env_rem_fids
+    (fids : list (FunctionIdentifier * FunctionExpression))
+    (env : Environment)
+    : Environment
+    :=
+  env_rem (map inr (map fst fids)) env.
+
+
+
+  Definition env_rem_fids_vars
+    (fids : list (FunctionIdentifier * FunctionExpression))
+    (vars : list Var)
+    (env : Environment)
+    : Environment
+    :=
+  env_rem_fids fids (env_rem_vars vars env).
+
+
+
+  Definition env_rem_ext
+    (ext : list (nat * FunctionIdentifier * FunctionExpression))
+    (env : Environment)
+    : Environment
+    :=
+  env_rem (map inr (map snd (map fst ext))) env.
+
+
+
+End Main.
