src/Equivalence/BigStepToFrameStack/Simple/SubstituteLemmas.v
@@ -1,0 +1,269 @@
+From CoreErlang.Equivalence.BigStepToFrameStack.Simple Require Export Substitute.
+
+Import BigStep.
+
+Lemma foldl_ext :
+  forall (A B : Type) (f1 f2 : A -> B -> A) (x1 x2 : A) (l1 l2 : list B),
+    (forall (a : A) (b : B), f1 a b = f2 a b) ->
+    l1 = l2 ->
+    x1 = x2 ->
+    fold_left f1 l1 x1 = fold_left f2 l2 x2.
+Proof.
+  intros A B f1 f2 x1 x2 l1 l2 Hf Hl Hx.
+  rewrite Hl.
+  rewrite Hx.
+  clear Hl Hx l1 x1.
+  rename l2 into l.
+  rename x2 into x.
+  revert x.
+  induction l as [| b l IHl]; intros x; simpl.
+  - reflexivity.
+  - rewrite Hf.
+    by rewrite IHl.
+Qed.
+
+Lemma env_rem_fids_vars_empty_map :
+      forall (f : Environment -> Expression -> Expression) el,
+        map
+          (fun  '(fid, (vl, b)) =>
+            (fid, (vl, f (env_rem_fids_vars el vl []) b)))
+          el
+      = map
+          (fun '(fid, (vl, b)) =>
+            (fid, (vl, f [] b)))
+          el.
+    Proof.
+      intros.
+      apply map_ext.
+      intros [fid [vl b]].
+      by rewrite env_rem_fids_vars_empty.
+    Qed.
+
+Theorem subst_env_empty :
+  forall n e,
+    subst_env n [] e = e.
+Proof.
+  intros.
+  generalize dependent n.
+  induction e using derived_Expression_ind.
+  * (* Values *)
+    rename H into HForall.
+    induction el as [| e el IHel]; intros; destruct n; cbn.
+    1-3: reflexivity.
+    inv HForall.
+    rename H1 into He.
+    rename H2 into HForall.
+    specialize (IHel HForall (S n)).
+    clear HForall.
+    cbn.
+    f_equal.
+    rewrite He.
+    clear He.
+    cbn in IHel.
+    injection IHel; intros Hel.
+    clear IHel.
+    rewrite Hel.
+    reflexivity.
+  * destruct n; by cbn.
+  * destruct n; by cbn.
+  * destruct n; by cbn.
+  * destruct n; by cbn.
+  * (* Fun *)
+    destruct n; cbn.
+    - reflexivity.
+    - specialize (IHe n).
+      rewrite IHe.
+      reflexivity.
+  * (* Cons *)
+    destruct n; cbn.
+    - reflexivity.
+    - specialize (IHe1 n).
+      specialize (IHe2 n).
+      rewrite IHe1.
+      rewrite IHe2.
+      reflexivity.
+  * (* Tuple *)
+    rename H into HForall.
+    induction l as [| e el IHel]; intros; destruct n; cbn.
+    1-3: reflexivity.
+    inv HForall.
+    rename H1 into He.
+    rename H2 into HForall.
+    specialize (IHel HForall (S n)).
+    clear HForall.
+    cbn.
+    f_equal.
+    rewrite He.
+    clear He.
+    cbn in IHel.
+    injection IHel; intros Hel.
+    clear IHel.
+    rewrite Hel.
+    reflexivity.
+  * (* Call *)
+    rename H into HForall.
+    induction l as [| e el IHel]; intros; destruct n; cbn.
+    2: rewrite IHe1; by rewrite IHe2.
+    1-2: reflexivity.
+    rewrite IHe1.
+    rewrite IHe2.
+    inv HForall.
+    rename H1 into He.
+    rename H2 into HForall.
+    specialize (IHel HForall (S n)).
+    clear HForall.
+    cbn.
+    f_equal.
+    rewrite He.
+    clear He.
+    cbn in IHel.
+    injection IHel; intros Hel.
+    clear IHel.
+    rewrite Hel.
+    reflexivity.
+  * (* PrimOp *)
+    rename H into HForall.
+    induction l as [| e el IHel]; intros; destruct n; cbn.
+    1-3: reflexivity.
+    inv HForall.
+    rename H1 into He.
+    rename H2 into HForall.
+    specialize (IHel HForall (S n)).
+    clear HForall.
+    cbn.
+    f_equal.
+    rewrite He.
+    clear He.
+    cbn in IHel.
+    injection IHel; intros Hel.
+    clear IHel.
+    rewrite Hel.
+    reflexivity.
+  * (* App *)
+    rename e into e'.
+    rename H into HForall.
+    induction l as [| e el IHel]; intros; destruct n; cbn.
+    2: by rewrite IHe.
+    1-2: reflexivity.
+    inv HForall.
+    rename H1 into He.
+    rename H2 into HForall.
+    specialize (IHel HForall (S n)).
+    clear HForall.
+    cbn in IHel.
+    inv IHel.
+    clear H0.
+    rename H1 into Hel.
+    rewrite IHe.
+    rewrite IHe.
+    rewrite He.
+    rewrite Hel.
+    rewrite Hel.
+    reflexivity.
+  * (* Case *)
+    rename e into e'.
+    rename H into HForall.
+    induction l as [| e el IHel]; intros; destruct n; cbn.
+    2: by rewrite IHe.
+    1-2: reflexivity.
+    inv HForall.
+    destruct e as [e e2].
+    destruct e as [p e1].
+    destruct H1.
+    cbn in *.
+    rename H into He1.
+    rename H0 into He2.
+    rename H2 into HForall.
+    specialize (IHel HForall (S n)).
+    clear HForall IHe.
+    cbn in IHel.
+    injection IHel; intros Hel He.
+    clear IHel.
+    rewrite He.
+    rewrite Hel.
+    rewrite He1.
+    rewrite He2.
+    reflexivity.
+  * (* Let *)
+    destruct n; cbn.
+    - reflexivity.
+    - rewrite env_rem_vars_empty.
+      rewrite IHe1.
+      rewrite IHe2.
+      reflexivity.
+  * (* Seq *)
+    destruct n; cbn.
+    - reflexivity.
+    - rewrite IHe1.
+      rewrite IHe2.
+      reflexivity.
+  * (* LetRec *)
+    rename e into e'.
+    rename H into HForall.
+    induction l as [| e el IHel]; intros; destruct n.
+    2: cbn; by rewrite IHe.
+    1-2: reflexivity.
+    inv HForall.
+    destruct e as [f e].
+    destruct e as [l e].
+    cbn in H1.
+    rename H1 into He.
+    rename H2 into HForall.
+    specialize (IHel HForall (S n)).
+    clear HForall.
+    cbn in IHel.
+    injection IHel; intros Hefid Hel.
+    clear IHel.
+    simpl.
+    rewrite env_rem_fids_empty.
+    rewrite IHe.
+    rewrite env_rem_fids_vars_empty.
+    rewrite He.
+    cbn.
+    (*rewrite env_rem_fids_vars_empty_map in Hel. *)
+    f_equal.
+    f_equal.
+    rewrite <- Hel at 2.
+    apply map_ext.
+    intros [fid [vl b]].
+    rewrite env_rem_vars_empty.
+    cbn.
+    f_equal.
+    f_equal.
+    f_equal.
+    unfold env_rem_fids_vars.
+    unfold env_rem_fids.
+    unfold env_rem.
+    f_equal.
+    rewrite env_rem_vars_empty.
+    reflexivity.
+  * (* Map *)
+    rename H into HForall.
+    induction l as [| e el IHel]; intros; destruct n; cbn.
+    1-3: reflexivity.
+    inv HForall.
+    destruct e as [e1 e2].
+    destruct H1.
+    rename H into He1.
+    rename H0 into He2.
+    rename H2 into HForall.
+    specialize (IHel HForall (S n)).
+    clear HForall.
+    cbn.
+    f_equal.
+    rewrite He1.
+    rewrite He2.
+    clear He1 He2.
+    cbn in *.
+    injection IHel; intros Hel.
+    clear IHel.
+    rewrite Hel.
+    reflexivity.
+  * (* Try *)
+    destruct n; cbn.
+    - reflexivity.
+    - rewrite IHe1.
+      rewrite IHe2.
+      rewrite IHe3.
+      reflexivity.
+Qed.
